Developed until Simulation.v

src/tutorial/Example1.v
@@ -6,50 +6,84 @@ From Tutorial Require Import Imp FiniteSimulation.
 
 Set Implicit Arguments.
 
-Section EX.
+Section DEMO.
   (** We will prove that src refines tgt, using the finite simulation. *)
 
   Definition src0 : com := <{ ret 0 }>.
 
   Definition tgt0 : com := <{ "x" := (1 + 1); "y" := (2 * 1 - "x"); ret "y" }>.
 
-  Goal refines (Imp_STS1 tgt0) (Imp_STS1 src0).
+  Goal refines (Imp_Program1 src0) (Imp_Program1 tgt0).
   Proof.
-    apply adequacy. unfold simulation, Imp_STS1, src0, tgt0. ss. unfold Imp_init.
+    apply adequacy. unfold simulation, Imp_Program1, Imp_STS1, src0, tgt0, Imp_init. ss.
     (* Same as 'econstructor 4.' or 'eapply sim_silentT.' *)
     econs 4.
     { ss. }
-    ss. i. inv H. ss. split; auto.
+    ss. i. inv H.
+    (* We have two cases: 1. normal step, 2. step is not defined. 
+       Step is defined for this case, so the second case is trivially solved. 
+     *)
+    2:{ exfalso. eapply UNDEF. repeat econs. }
+    inv STEP. ss. split; auto.
     econs 4.
     { ss. }
-    ss. i. inv H. ss. split; auto.
-    inv H7. inv H4. inv H5. ss.
-    econs 4.
-    { ss. }
-    ss. i. inv H. ss. split; auto.
-    econs 4.
-    { ss. }
-    ss. i. inv H. ss. split; auto.
-    econs 4.
-    { ss. }
-    ss. i. inv H. ss. split; auto.
-    inv H7. inv H4. inv H5. inv H6. inv H7. inv H1. ss.
-    econs 4.
-    { ss. }
-    ss. i. inv H. ss. split; auto.
+    ss. i. inv H.
+    2:{ exfalso. eapply UNDEF. repeat econs. }
+    inv STEP. ss. split; auto.
+    (* As you can see, simulation proofs can get very length.
+       Thus one usually defines a tactic that automatically takes care of trivial steps.
+       So let us define some simple tactics first.
+     *)
+  Abort.
+
+  (** Note that a tactic defined inside a section can only be used in that section, in general. *)
+
+  (* Solves tgt undef case if tgt is not undef. *)
+  Ltac solve_tgt_ub := 
+    exfalso;
+    match goal with
+    | [UNDEF : forall _ _, ~ (ceval _ _ _) |- _] => eapply UNDEF
+    end;
+    repeat econs.
+
+  (* Makes a tgt step. *)
+  Ltac step_tgt_silent0 :=
+    match goal with
+    | [STEP: ceval _ _ _ |- _] => inv STEP
+    end;
+    ss; split; auto.
+
+  (* Combines above two tactics. *)
+  Ltac step_tgt_silent :=
+    try (econs 4;
+         [ss
+         | ss; intros ev st_tgt1 STEP0; inv STEP0;
+           [step_tgt_silent0 | solve_tgt_ub]
+        ]).
+
+  Goal refines (Imp_Program1 src0) (Imp_Program1 tgt0).
+  Proof.
+    apply adequacy. unfold simulation, Imp_Program1, Imp_STS1, src0, tgt0, Imp_init. ss.
+    step_tgt_silent.
+    step_tgt_silent.
+    inv H6. inv H4. inv H5. ss.
+    (* We can take multiple steps like this: *)
+    do 3 step_tgt_silent.
+    inv H6. inv H4. inv H5. inv H6. inv H7. inv H1. ss.
+    step_tgt_silent.
     (* Now evaluate return commands. 
        When both src and tgt needs to progress, usually taking tgt step first is better;
        we are usually proving 'forall tgt event, exists src event'.
      *)
-    econs 4.
-    { ss. }
-    ss. i. inv H. ss. split; auto.
-    inv H6. inv H1.
+    step_tgt_silent.
+    inv H5. inv H1.
+    (* Now take src step. *)
     econs 3.
     { ss. }
     ss. exists (inr LInternal). eexists. split.
-    { econs. econs.
-      (* Coq detects correct constructors for this: 'eapply E_Ret. eapply E_ANum.'. *)
+    { econs. econs. econs.
+      (* Coq detects correct constructors for this case.
+         Same as 'eapply Step_normal. eapply E_Ret. eapply E_ANum.'. *)
     }
     ss. split; auto.
     (* There is only one possible constructor for this: 'sim_term'. *)
@@ -59,74 +93,29 @@ Section EX.
     { auto. }
   Qed.
 
-  (* Simulation proofs can be very length, as you can see from this simple example.
-     Thus one usually define a tactic that automatically take care of trivial steps.
-     Our examples will be simple enough, so you can define yours if you need.
-     Note that a tactic defined inside a section can only be used in that section in general.
-   *)
-
-  Ltac step_tgt_silents :=
-    try (econs 4; [ss | ss; intros ev st_tgt1 STEP; inv STEP; ss; split; auto]).
-
-  Goal refines (Imp_STS1 tgt0) (Imp_STS1 src0).
-  Proof.
-    apply adequacy. unfold simulation, Imp_STS1, src0, tgt0. ss. unfold Imp_init.
-    do 2 step_tgt_silents.
-    inv H6. inv H4. inv H5. ss.
-    do 3 step_tgt_silents.
-    inv H6. inv H4. inv H5. inv H6. inv H7. inv H1. ss.
-    do 2 step_tgt_silents.
-    inv H5. inv H1.
-    econs 3.
-    { ss. }
-    ss. exists (inr LInternal). eexists. split.
-    { econs. econs. }
-    ss. split; auto.
-    econs.
-    { simpl. eauto. }
-    { simpl. eauto. }
-    { auto. }
-  Qed.
-
-End EX.
+End DEMO.
 
 Section EX.
-  (** Prove the following refinements. *)
+  (** Prove the following refinements. Develop tactics to simplify the proofs. *)
 
-  (* Ex1. If a loop is guaranteed to terminate, we can prove it by induction. *)
-
-  Definition src1 : com := <{ ret 0 }>.
+  (* Ex1. Interactions with the external world is observable, so should be preserved. *)
+  Definition src1 : com := <{ "a" :=@ "print" <[0 : aexp]>; ret "a" }>.
 
   Definition tgt1 : com :=
-    <{ "x" := 100;
-       while ("x")
-       do ("x" := ("x" - 1))
-       end;
-       ret "x"
-    }>.
-
-  Goal refines (Imp_STS1 tgt1) (Imp_STS1 src1).
-  Proof.
-  Admitted.
-
-  (* Ex2. Interactions with the external world is observable, so should be preserved. *)
-
-  Definition src2 : com := <{ "a" :=@ "print" <[0 : aexp]>; ret "a" }>.
-
-  Definition tgt2 : com :=
     <{ "x" := 0; "y" :=@ "print" <["x" : aexp]>; ret "y" }>.
 
-  Goal refines (Imp_STS1 tgt2) (Imp_STS1 src2).
+  Goal refines (Imp_Program1 src1) (Imp_Program1 tgt1).
   Proof.
   Admitted.
 
-  (* Ex3. If semantics is given by Imp_STS1, memory accesses are also observable. *)
-  Definition src3 : com := <{ &<1> := 5; "a" := &<1>; ret "a" }>.
 
-  Definition tgt3 : com :=
+  (* Ex2. If semantics is given by Imp_STS1, memory accesses are also observable. *)
+  Definition src2 : com := <{ &<1> := 5; "a" := &<1>; ret "a" }>.
+
+  Definition tgt2 : com :=
     <{ "x" := 2; &<1> := ("x" + 3); "y" := &<1>; ret "y" }>.
 
-  Goal refines (Imp_STS1 tgt3) (Imp_STS1 src3).
+  Goal refines (Imp_Program1 src2) (Imp_Program1 tgt2).
   Proof.
   Admitted.
 
@@ -134,9 +123,33 @@ Section EX.
      we do not want to keep memory accesses visible.
      Imp_STS2 is the right semantics for this. 
    *)
-  Definition src3' : com := <{ ret 5 }>.
+  Definition src2' : com := <{ ret 5 }>.
 
-  Goal refines (Imp_STS2 tgt3) (Imp_STS2 src3').
+  Goal refines (Imp_Program2 src2') (Imp_Program2 tgt2).
+  Proof.
+  Admitted.
+
+
+  (* Ex3. If the source program can exhibit undefined behavior, refinement always holds. *)
+  Definition src3 : com := <{ ret "a" }>.
+
+  Goal forall tgt, refines (Imp_Program1 src3) (Imp_Program1 tgt).
+  Proof.
+  Admitted.
+
+
+  (* Ex4. If a loop always terminates, we can prove it by induction. *)
+  Definition src4 : com := <{ ret 0 }>.
+
+  Definition tgt4 : com :=
+    <{ "x" := 100;
+       while ("x")
+       do ("x" := ("x" - 1))
+       end;
+       ret "x"
+    }>.
+
+  Goal refines (Imp_Program1 src4) (Imp_Program1 tgt4).
   Proof.
   Admitted.
 
@@ -145,40 +158,12 @@ End EX.
 Section DIV.
   (** Simulation in current form can't prove refinement between possibly diverging programs. *)
 
-  (* Ex4. We can prove the following refinement, which always terminates. *)
-
-  Definition src4 : com :=
-    <{ "x" := 100;
-       while ("x")
-       do ("a" :=@ "print" <["x" : aexp]>;
-           "x" := ("x" - 1))
-       end;
-       ret "x"
-    }>.
-
-  Definition tgt4 : com :=
-    <{ "x" := 100;
-       while ("x")
-       do ("a" :=@ "print" <["x" : aexp]>;
-           "x" := ("x" - 1))
-       end;
-       ret "x"
-    }>.
-
-  Goal refines (Imp_STS2 tgt4) (Imp_STS2 src4).
-  Proof.
-  Admitted.
-
-  (* Ex5. However, we can't prove the following refinement, because it can diverge.
-     Also note that even though src5 and tgt5 are the same programs 
-     (thus trivially refines each other), our simulation relation is too weak to prove this.
-     Compare this with Ex1 and Ex4.
-   *)
-
+  (* DIV1. We can prove the following refinement, which always terminates. *)
   Definition src5 : com :=
     <{ "x" := 100;
        while ("x")
-       do ("x" := AAny)
+       do ("a" :=@ "print" <["x" : aexp]>;
+           "x" := ("x" - 1))
        end;
        ret "x"
     }>.
@@ -186,24 +171,41 @@ Section DIV.
   Definition tgt5 : com :=
     <{ "x" := 100;
        while ("x")
+       do ("a" :=@ "print" <["x" : aexp]>;
+           "x" := ("x" - 1))
+       end;
+       ret "x"
+    }>.
+
+  Goal refines (Imp_Program2 src5) (Imp_Program2 tgt5).
+  Proof.
+  Admitted.
+
+
+  (* DIV2. However, we can't prove the following refinement because it can diverge.
+     Also note that even though src5 and tgt5 are the same programs 
+     (thus trivially refines each other), our simulation relation is too weak to prove this.
+     Compare this with Ex1 and Ex4.
+   *)
+  Definition src6 : com :=
+    <{ "x" := 100;
+       while ("x")
        do ("x" := AAny)
        end;
        ret "x"
     }>.
 
-  Goal refines (Imp_STS2 tgt5) (Imp_STS2 src5).
+  Definition tgt6 : com :=
+    <{ "x" := 100;
+       while ("x")
+       do ("x" := AAny)
+       end;
+       ret "x"
+    }>.
+
+  Goal refines (Imp_Program2 src6) (Imp_Program2 tgt6).
   Proof.
-    (* We can't prove this right now. *)
+  (* We can't prove this right now. Try to prove using induction, and see where it fails. *)
   Abort.
 
 End DIV.
-
-Section SIM.
-  (** We will define a simulation relation that can work with diverging programs.
-      These simulations are called 'termination sensitive' or 'termination preserving'.
-   *)
-
-  (* Our first attempt. *)
-
-
-End SIM.
