src/tutorial/FiniteSimulation.v
@@ -7,56 +7,54 @@ Set Implicit Arguments.
 Section SIM.
 
   Context {event: Event}.
-  Context {src: @STS event}.
-  Context {tgt: @STS event}.
+  Context {sem: @STS event}.
 
   Notation ekind := event.(label_kind).
-  Notation ssort := src.(state_sort).
-  Notation tsort := tgt.(state_sort).
+  Notation sort := sem.(state_sort).
 
   Inductive sim
             (RR: Z -> Z -> Prop)
     :
-    src.(state) -> tgt.(state) -> Prop :=
+    sem.(state) -> sem.(state) -> Prop :=
   | sim_term
       st_src st_tgt r_src r_tgt
-      (TERMS: ssort st_src = final r_src)
-      (TERMT: tsort st_tgt = final r_tgt)
+      (TERMS: sort st_src = final r_src)
+      (TERMT: sort st_tgt = final r_tgt)
       (SIM: RR r_src r_tgt)
     :
     sim RR st_src st_tgt
   | sim_obs
       st_src0 st_tgt0
-      (OBSS: ssort st_src0 = normal)
-      (OBST: tsort st_tgt0 = normal)
+      (OBSS: sort st_src0 = normal)
+      (OBST: sort st_tgt0 = normal)
       (SIM: forall ev st_tgt1,
-          (tgt.(step) st_tgt0 ev st_tgt1) ->
+          (sem.(step) st_tgt0 ev st_tgt1) ->
           (ekind ev = observableE) /\
-          exists st_src1, (src.(step) st_src0 ev st_src1) /\
+          exists st_src1, (sem.(step) st_src0 ev st_src1) /\
                        (sim RR st_src1 st_tgt1))
     :
     sim RR st_src0 st_tgt0
   | sim_silentS
       st_src0 st_tgt
-      (SORT: ssort st_src0 = normal)
+      (SORT: sort st_src0 = normal)
       (SIM: exists ev st_src1,
-          (src.(step) st_src0 ev st_src1) /\
+          (sem.(step) st_src0 ev st_src1) /\
             (ekind ev = silentE) /\
             (sim RR st_src1 st_tgt))
     :
     sim RR st_src0 st_tgt
   | sim_silentT
       st_src st_tgt0
-      (SORT: tsort st_tgt0 = normal)
+      (SORT: sort st_tgt0 = normal)
       (SIM: forall ev st_tgt1,
-          (tgt.(step) st_tgt0 ev st_tgt1) ->
+          (sem.(step) st_tgt0 ev st_tgt1) ->
           (ekind ev = silentE) /\
           (sim RR st_src st_tgt1))
     :
     sim RR st_src st_tgt0
   | sim_ub
       st_src st_tgt
-      (SORT: ssort st_src = undef)
+      (SORT: sort st_src = undef)
     :
     sim RR st_src st_tgt
   .
@@ -64,41 +62,41 @@ Section SIM.
   (* Coq fails to generate a correct induction lemma. *)
   Lemma sim_ind2
         (RR: Z -> Z -> Prop)
-        (P: src.(state) -> tgt.(state) -> Prop)
+        (P: sem.(state) -> sem.(state) -> Prop)
         (TERM: forall st_src st_tgt r_src r_tgt
-                 (TERMS: ssort st_src = final r_src)
-                 (TERMT: tsort st_tgt = final r_tgt)
+                 (TERMS: sort st_src = final r_src)
+                 (TERMT: sort st_tgt = final r_tgt)
                  (SIM: RR r_src r_tgt)
           ,
             P st_src st_tgt)
         (OBS: forall st_src0 st_tgt0
-                (OBSS: ssort st_src0 = normal)
-                (OBST: tsort st_tgt0 = normal)
+                (OBSS: sort st_src0 = normal)
+                (OBST: sort st_tgt0 = normal)
                 (SIM: forall ev st_tgt1,
-                    (tgt.(step) st_tgt0 ev st_tgt1) ->
+                    (sem.(step) st_tgt0 ev st_tgt1) ->
                     (ekind ev = observableE) /\
-                    exists st_src1, (src.(step) st_src0 ev st_src1) /\
+                    exists st_src1, (sem.(step) st_src0 ev st_src1) /\
                                  (sim RR st_src1 st_tgt1) /\ (P st_src1 st_tgt1))
           ,
             P st_src0 st_tgt0)
         (SILENTS: forall st_src0 st_tgt
-                    (SORT: ssort st_src0 = normal)
+                    (SORT: sort st_src0 = normal)
                     (SIM: exists ev st_src1,
-                        (src.(step) st_src0 ev st_src1) /\
+                        (sem.(step) st_src0 ev st_src1) /\
                           (ekind ev = silentE) /\
                           (sim RR st_src1 st_tgt) /\ (P st_src1 st_tgt))
           ,
             P st_src0 st_tgt)
         (SILENTT: forall st_src st_tgt0
-                    (SORT: tsort st_tgt0 = normal)
+                    (SORT: sort st_tgt0 = normal)
                     (SIM: forall ev st_tgt1,
-                        (tgt.(step) st_tgt0 ev st_tgt1) ->
+                        (sem.(step) st_tgt0 ev st_tgt1) ->
                         (ekind ev = silentE) /\
                         ((sim RR st_src st_tgt1) /\ (P st_src st_tgt1)))
           ,
             P st_src st_tgt0)
         (UB: forall st_src st_tgt
-               (UB: ssort st_src = undef)
+               (UB: sort st_src = undef)
           ,
             P st_src st_tgt)
     :
@@ -117,18 +115,18 @@ Section SIM.
 End SIM.
 #[export] Hint Constructors sim: core.
 
-Definition simulation {l: Event} (src tgt: @STS l) := sim (@eq Z) src.(init) tgt.(init).
+Definition simulation {l: Event} {sem: @STS l} (src tgt: Program sem) :=
+  sim (@eq Z) src.(init) tgt.(init).
 
 Section ADEQ.
 
   Context {event: Event}.
-  Context {src: @STS event}.
-  Context {tgt: @STS event}.
+  Context {sem: @STS event}.
 
   Lemma adequacy_spin
         (RR: Z -> Z -> Prop)
-        (st_src: src.(state))
-        (st_tgt: tgt.(state))
+        (st_src: sem.(state))
+        (st_tgt: sem.(state))
         (SIM: sim RR st_src st_tgt)
         (SPIN: diverge st_tgt)
     :
@@ -149,8 +147,8 @@ Section ADEQ.
   Qed.
 
   Lemma adequacy_aux
-        (st_src0: src.(state))
-        (st_tgt0: tgt.(state))
+        (st_src0: sem.(state))
+        (st_tgt0: sem.(state))
         (SIM: sim eq st_src0 st_tgt0)
     :
     forall tr, (behavior st_tgt0 tr) -> (behavior st_src0 tr).
@@ -186,9 +184,10 @@ Section ADEQ.
   Qed.
 
   Theorem adequacy
+          (src tgt: Program sem)
           (SIM: simulation src tgt)
     :
-    refines tgt src.
+    refines src tgt.
   Proof.
     ii. eapply adequacy_aux; eauto.
   Qed.
