src/tutorial/Refinement.v
@@ -6,18 +6,18 @@ From Coq Require Export ZArith.
 Set Implicit Arguments.
 Open Scope Z_scope.
 
-(* Program refinement is an approach in program verification, 
+(** Program refinement is an approach in program verification, 
    where one verifies that every possible behavior of a program 
    (called the target or the implementation) 
    is also possible by another program (called the source or the spec).
    Usually, behavior of a program is defined as a set of traces, 
    where a trace is a stream of observable events of a program, 
-   including divergence (infinite silent execution), termination, and error.
-   Observable events can differ by what one wants to verify.
-*)
+   including divergence (infinite silent execution) and termination.
+   Observable events are user-defined; a usual example is system calls.
+ *)
 
-(* We first define the trace. *)
 Section TRACE.
+  (** We first define the trace. *)
 
   Context {event: Type}.
 
@@ -34,9 +34,10 @@ Section TRACE.
 
 End TRACE.
 
-(* We assume a simple labeled state transition system. *)
 Section STS.
+  (** We define semantics of programs using a simple labeled state transition system. *)
 
+  (** We assume two kinds of events, silent and observable. *)
   Variant kind: Type :=
     | silentE
     | observableE
@@ -48,6 +49,9 @@ Section STS.
         label_kind: label -> kind;
       }.
 
+  (** We assume that a state can be classified into 
+      normal, final (no more steps), or undef ('transition is undefined') 
+   *)
   Variant sort: Type :=
     | normal
     | final (retv: Z)
@@ -57,12 +61,13 @@ Section STS.
   Record STS {e: Event}: Type :=
     mk_sts {
         state: Type;
-        init: state;
-        (* Note that step is a relation, not a function. In general, program execution can be non-deterministic. *)
+        (* Note that we assume that step is a relation, 
+           in order to allow for nondeterminism. *)
         step: state -> e.(label) -> state -> Prop;
         state_sort: state -> sort;
       }.
 
+  (* Properties we assume for a STS, as a part of specification. *)
   Record STS_valid (e: Event) (s: @STS e): Prop :=
     mk_sts_valid {
         normal_valid:
@@ -78,21 +83,29 @@ Section STS.
                forall ev st1, (~ s.(step) st0 ev st1);
       }.
 
+  (** A program simply specifies an initial state. *)
+  Record Program {e: Event} (sem: @STS e): Type :=
+    mk_program {
+        init: sem.(state)
+      }.
+
 End STS.
 
-(* We now define the behavior of a STS. *)
 Section BEH.
+  (** We now define the behavior of a STS. *)
 
-  Context {event: Event}.
-  Local Notation event := event.(event).
-  Local Notation ekind := event.(label_kind).
+  Context {ev: Event}.
+  Local Notation event := ev.(label).
+  Local Notation ekind := ev.(label_kind).
 
-  Context {prog: @STS event}.
-  Local Notation state := prog.(state).
-  Local Notation init := prog.(init).
-  Local Notation step := prog.(step).
-  Local Notation ssort := prog.(state_sort).
+  Context {sem: @STS ev}.
+  Local Notation state := sem.(state).
+  Local Notation step := sem.(step).
+  Local Notation ssort := sem.(state_sort).
 
+  (** We use the paco libray to define coinductive properties.
+      'diverge' states that a state makes infinite silent transitions, or it is undefined.
+   *)
   Variant _diverge
           (diverge: state -> Prop)
     :
@@ -119,7 +132,7 @@ Section BEH.
   Proof.
     ii. inv IN.
     - econs 1; eauto.
-      (* eapply diverge_silent; eauto. *)
+      (* Same as 'eapply diverge_silent; eauto.'. *)
     - econs 2; eauto.
   Qed.
 
@@ -128,9 +141,11 @@ Section BEH.
   Hint Resolve diverge_mon: paco.
   Hint Resolve cpn1_wcompat: paco.
 
-  (* Behavior is a mixed inductive-coinductive definition.
-     Inductive because we only want finite number of silent steps (infinite silent step case is treated as divergence).
-  *)
+  (** Behavior is a mixed inductive-coinductive definition.
+      Specifically, silent steps are allowed only finite times using inductive definition ('_behavior')
+      (infinite silent steps case is treated as divergence),
+      and observable events are allowed infinitely many times ('behavior').
+   *)
   Inductive _behavior
             (behavior: state -> trace -> Prop)
     :
@@ -142,6 +157,7 @@ Section BEH.
     _behavior behavior st (term retv)
   | beh_spin
       st
+      (* Diverge case is separately defined. *)
       (SPIN: diverge st)
     :
     _behavior behavior st spin
@@ -150,12 +166,12 @@ Section BEH.
       (SORT: ssort st = undef)
     :
     _behavior behavior st tr
-  (* Silent case is inductive. *)
   | beh_silent
       st0 ev st1 tr
       (SORT: ssort st0 = normal)
       (KIND: ekind ev = silentE)
       (STEP: step st0 ev st1)
+      (* Silent case is inductive. *)
       (NEXT: _behavior behavior st1 tr)
     :
     _behavior behavior st0 tr
@@ -164,6 +180,7 @@ Section BEH.
       (SORT: ssort st0 = normal)
       (KIND: ekind ev = observableE)
       (STEP: step st0 ev st1)
+      (* Observable case is coinductive. *)
       (NEXT: behavior st1 tl)
     :
     _behavior behavior st0 (cons (obs ev) tl)
@@ -171,6 +188,7 @@ Section BEH.
 
   Definition behavior: state -> trace -> Prop := paco2 _behavior bot2.
 
+  (* Boilerplate code for paco. *)
   Lemma behavior_mon: monotone2 _behavior.
   Proof.
     ii. induction IN; eauto.
@@ -186,6 +204,7 @@ Section BEH.
   Hint Resolve behavior_mon: paco.
   Hint Resolve cpn2_wcompat: paco.
 
+  (* A more convenient induction. *)
   Lemma behavior_ind:
     forall (P: state -> trace -> Prop)
   (TERM: forall st retv
@@ -222,7 +241,10 @@ Section BEH.
     - punfold H.
   Qed.
 
-  (* Upto properties. *)
+  (* Upto properties.
+     These lemmas simplify coinductive proofs involving 'behavior'.
+     You don't need to understand them for now.
+   *)
 
   Variant behavior_indC
           (behavior: state -> trace -> Prop)
@@ -293,13 +315,15 @@ End BEH.
 #[global] Hint Resolve cpn2_wcompat: paco.
 
 Section REF.
+  (** Refinement is simply a set inclusion. *)
 
   Context {event: Event}.
+  Context {sem: @STS event}.
 
-  (* Refinement is set inclusion, thus transitive. *)
-  Definition refines (tgt src: @STS event): Prop :=
+  Definition refines (src tgt: Program sem): Prop :=
     forall tr, (behavior tgt.(init) tr) -> (behavior src.(init) tr).
 
+  (* Refinement is trivially transitive. *)
   Lemma refines_trans: Transitive refines.
   Proof.
     ii. unfold refines in *. eauto.
