src/tutorial/Simulation.v
@@ -5,59 +5,70 @@ From Tutorial Require Import Refinement.
 Set Implicit Arguments.
 
 Section SIM.
+  (** We define a sound simulation. 
+      There are many styles in defining a termination sensitive simulation,
+      and we follow the one presented in:
+      Stuttering for Free (Cho et al., OOPSLA'23, https://doi.org/10.1145/3622857).
+   *)
 
   Context {event: Event}.
-  Context {src: @STS event}.
-  Context {tgt: @STS event}.
+  Context {sem: @STS event}.
 
   Notation ekind := event.(label_kind).
-  Notation ssort := src.(state_sort).
-  Notation tsort := tgt.(state_sort).
+  Notation sort := sem.(state_sort).
 
+  (** This simulation ensures *finite* stuttering by allowing src/tgt to stutter only inductively.
+      One can see that each constructors taking steps are defined inductively with '_sim'.
+      However, unlike the finite simulation, this sim is equipped with two Boolean flags, 
+      which are set to true when src/tgt side makes progress (i.e. takes a step).
+      Then coinductive progress is only allowed when both flags are true (sim_progress).
+      In other words, if one wants to prove by coinduction, 
+      one must show that both the src and the tgt already made progress.
+   *)
   Inductive _sim
-            (sim: forall (RR: Z -> Z -> Prop), bool -> bool -> src.(state) -> tgt.(state) -> Prop)
+            (sim: forall (RR: Z -> Z -> Prop), bool -> bool -> sem.(state) -> sem.(state) -> Prop)
             (RR: Z -> Z -> Prop) (p_src p_tgt: bool)
     :
-    src.(state) -> tgt.(state) -> Prop :=
+    sem.(state) -> sem.(state) -> Prop :=
   | sim_term
       st_src st_tgt r_src r_tgt
-      (TERMS: ssort st_src = final r_src)
-      (TERMT: tsort st_tgt = final r_tgt)
+      (TERMS: sort st_src = final r_src)
+      (TERMT: sort st_tgt = final r_tgt)
       (SIM: RR r_src r_tgt)
     :
     _sim sim RR p_src p_tgt st_src st_tgt
   | sim_obs
       st_src0 st_tgt0
-      (OBSS: ssort st_src0 = normal)
-      (OBST: tsort st_tgt0 = normal)
+      (OBSS: sort st_src0 = normal)
+      (OBST: sort st_tgt0 = normal)
       (SIM: forall ev st_tgt1,
-          (tgt.(step) st_tgt0 ev st_tgt1) ->
+          (sem.(step) st_tgt0 ev st_tgt1) ->
           (ekind ev = observableE) /\
-          exists st_src1, (src.(step) st_src0 ev st_src1) /\
+          exists st_src1, (sem.(step) st_src0 ev st_src1) /\
                        (_sim sim RR true true st_src1 st_tgt1))
     :
     _sim sim RR p_src p_tgt st_src0 st_tgt0
   | sim_silentS
       st_src0 st_tgt
-      (SORT: ssort st_src0 = normal)
+      (SORT: sort st_src0 = normal)
       (SIM: exists ev st_src1,
-          (src.(step) st_src0 ev st_src1) /\
+          (sem.(step) st_src0 ev st_src1) /\
             (ekind ev = silentE) /\
             (_sim sim RR true p_tgt st_src1 st_tgt))
     :
     _sim sim RR p_src p_tgt st_src0 st_tgt
   | sim_silentR
       st_src st_tgt0
-      (SORT: tsort st_tgt0 = normal)
+      (SORT: sort st_tgt0 = normal)
       (SIM: forall ev st_tgt1,
-          (tgt.(step) st_tgt0 ev st_tgt1) ->
+          (sem.(step) st_tgt0 ev st_tgt1) ->
           (ekind ev = silentE) /\
           (_sim sim RR p_src true st_src st_tgt1))
     :
     _sim sim RR p_src p_tgt st_src st_tgt0
   | sim_ub
       st_src st_tgt
-      (SORT: ssort st_src = undef)
+      (SORT: sort st_src = undef)
     :
     _sim sim RR p_src p_tgt st_src st_tgt
   | sim_progress
@@ -69,40 +80,40 @@ Section SIM.
     _sim sim RR p_src p_tgt st_src st_tgt.
 
   (* Coq fails to generate a correct induction lemma. *)
-  Lemma _sim_ind2 (sim: forall (RR: Z -> Z -> Prop), bool -> bool -> src.(state) -> tgt.(state) -> Prop)
+  Lemma _sim_ind2 (sim: forall (RR: Z -> Z -> Prop), bool -> bool -> sem.(state) -> sem.(state) -> Prop)
         (RR: Z -> Z -> Prop)
-        (P: bool -> bool -> src.(state) -> tgt.(state) -> Prop)
+        (P: bool -> bool -> sem.(state) -> sem.(state) -> Prop)
   (TERM: forall p_src p_tgt st_src st_tgt r_src r_tgt
-      (TERMS: ssort st_src = final r_src)
-      (TERMT: tsort st_tgt = final r_tgt)
+      (TERMS: sort st_src = final r_src)
+      (TERMT: sort st_tgt = final r_tgt)
       (SIM: RR r_src r_tgt)
     ,
     P p_src p_tgt st_src st_tgt)
   (OBS: forall p_src p_tgt st_src0 st_tgt0
-      (OBSS: ssort st_src0 = normal)
-      (OBST: tsort st_tgt0 = normal)
-      (SIM: forall ev st_tgt1, (tgt.(step) st_tgt0 ev st_tgt1) ->
+      (OBSS: sort st_src0 = normal)
+      (OBST: sort st_tgt0 = normal)
+      (SIM: forall ev st_tgt1, (sem.(step) st_tgt0 ev st_tgt1) ->
                           (ekind ev = observableE) /\
-                       exists st_src1, (src.(step) st_src0 ev st_src1) /\
+                       exists st_src1, (sem.(step) st_src0 ev st_src1) /\
                                     (_sim sim RR true true st_src1 st_tgt1) /\ (P true true st_src1 st_tgt1))
     ,
     P p_src p_tgt st_src0 st_tgt0)
   (SILENTL: forall p_src p_tgt st_src0 st_tgt
-      (SORT: ssort st_src0 = normal)
-      (SIM: exists ev st_src1, (src.(step) st_src0 ev st_src1) /\
+      (SORT: sort st_src0 = normal)
+      (SIM: exists ev st_src1, (sem.(step) st_src0 ev st_src1) /\
                             (ekind ev = silentE) /\
                        (_sim sim RR true p_tgt st_src1 st_tgt) /\ (P true p_tgt st_src1 st_tgt))
     ,
     P p_src p_tgt st_src0 st_tgt)
   (SILENTR: forall p_src p_tgt st_src st_tgt0
-      (SORT: tsort st_tgt0 = normal)
-      (SIM: forall ev st_tgt1, (tgt.(step) st_tgt0 ev st_tgt1) ->
+      (SORT: sort st_tgt0 = normal)
+      (SIM: forall ev st_tgt1, (sem.(step) st_tgt0 ev st_tgt1) ->
                           (ekind ev = silentE) /\
                        ((_sim sim RR p_src true st_src st_tgt1) /\ (P p_src true st_src st_tgt1)))
     ,
     P p_src p_tgt st_src st_tgt0)
   (UB: forall p_src p_tgt st_src st_tgt
-      (UB: ssort st_src = undef)
+      (UB: sort st_src = undef)
     ,
     P p_src p_tgt st_src st_tgt)
   (PROG: forall p_src p_tgt st_src st_tgt
@@ -125,8 +136,9 @@ Section SIM.
     - eapply PROG; eauto.
   Qed.
 
-  Definition sim: forall (RR: Z -> Z -> Prop), bool -> bool -> src.(state) -> tgt.(state) -> Prop := paco5 _sim bot5.
+  Definition sim: forall (RR: Z -> Z -> Prop), bool -> bool -> sem.(state) -> sem.(state) -> Prop := paco5 _sim bot5.
 
+  (* Boilerplate codes for paco. *)
   Lemma sim_mon: monotone5 _sim.
   Proof.
     ii. induction IN using _sim_ind2.
@@ -139,38 +151,38 @@ Section SIM.
   Qed.
 
   Lemma sim_ind (RR: Z -> Z -> Prop)
-        (P: bool -> bool -> src.(state) -> tgt.(state) -> Prop)
+        (P: bool -> bool -> sem.(state) -> sem.(state) -> Prop)
   (TERM: forall p_src p_tgt st_src st_tgt r_src r_tgt
-      (TERMS: ssort st_src = final r_src)
-      (TERMT: tsort st_tgt = final r_tgt)
+      (TERMS: sort st_src = final r_src)
+      (TERMT: sort st_tgt = final r_tgt)
       (SIM: RR r_src r_tgt)
     ,
     P p_src p_tgt st_src st_tgt)
   (OBS: forall p_src p_tgt st_src0 st_tgt0
-      (OBSS: ssort st_src0 = normal)
-      (OBST: tsort st_tgt0 = normal)
-      (SIM: forall ev st_tgt1, (tgt.(step) st_tgt0 ev st_tgt1) ->
+      (OBSS: sort st_src0 = normal)
+      (OBST: sort st_tgt0 = normal)
+      (SIM: forall ev st_tgt1, (sem.(step) st_tgt0 ev st_tgt1) ->
                           (ekind ev = observableE) /\
-                       exists st_src1, (src.(step) st_src0 ev st_src1) /\
+                       exists st_src1, (sem.(step) st_src0 ev st_src1) /\
                                     (sim RR true true st_src1 st_tgt1) /\ (P true true st_src1 st_tgt1))
     ,
     P p_src p_tgt st_src0 st_tgt0)
   (SILENTL: forall p_src p_tgt st_src0 st_tgt
-      (SORT: ssort st_src0 = normal)
-      (SIM: exists ev st_src1, (src.(step) st_src0 ev st_src1) /\
+      (SORT: sort st_src0 = normal)
+      (SIM: exists ev st_src1, (sem.(step) st_src0 ev st_src1) /\
                             (ekind ev = silentE) /\
                        (sim RR true p_tgt st_src1 st_tgt) /\ (P true p_tgt st_src1 st_tgt))
     ,
     P p_src p_tgt st_src0 st_tgt)
   (SILENTR: forall p_src p_tgt st_src st_tgt0
-      (SORT: tsort st_tgt0 = normal)
-      (SIM: forall ev st_tgt1, (tgt.(step) st_tgt0 ev st_tgt1) ->
+      (SORT: sort st_tgt0 = normal)
+      (SIM: forall ev st_tgt1, (sem.(step) st_tgt0 ev st_tgt1) ->
                           (ekind ev = silentE) /\
                        ((sim RR p_src true st_src st_tgt1) /\ (P p_src true st_src st_tgt1)))
     ,
     P p_src p_tgt st_src st_tgt0)
   (UB: forall p_src p_tgt st_src st_tgt
-      (UB: ssort st_src = undef)
+      (UB: sort st_src = undef)
     ,
     P p_src p_tgt st_src st_tgt)
   (PROG: forall p_src p_tgt st_src st_tgt
@@ -196,49 +208,52 @@ Section SIM.
   Hint Resolve sim_mon: paco.
   Hint Resolve cpn5_wcompat: paco.
 
-  (* Upto properties. *)
+  (** Upto properties.
+      These are useful for doing coinductive proofs with paco.
+      You don't need to understand them now; we will revisit them later.
+   *)
 
   Variant sim_indC
-          (sim: forall (RR: Z -> Z -> Prop), bool -> bool -> src.(state) -> tgt.(state) -> Prop)
+          (sim: forall (RR: Z -> Z -> Prop), bool -> bool -> sem.(state) -> sem.(state) -> Prop)
           (RR: Z -> Z -> Prop) p_src p_tgt
     :
-    src.(state) -> tgt.(state) -> Prop :=
+    sem.(state) -> sem.(state) -> Prop :=
     | sim_indC_term
         st_src st_tgt r_src r_tgt
-        (TERMS: ssort st_src = final r_src)
-        (TERMT: tsort st_tgt = final r_tgt)
+        (TERMS: sort st_src = final r_src)
+        (TERMT: sort st_tgt = final r_tgt)
         (SIM: RR r_src r_tgt)
       :
       sim_indC sim RR p_src p_tgt st_src st_tgt
     | sim_indC_obs
         st_src0 st_tgt0
-        (OBSS: ssort st_src0 = normal)
-        (OBST: tsort st_tgt0 = normal)
-        (SIM: forall ev st_tgt1, (tgt.(step) st_tgt0 ev st_tgt1) ->
+        (OBSS: sort st_src0 = normal)
+        (OBST: sort st_tgt0 = normal)
+        (SIM: forall ev st_tgt1, (sem.(step) st_tgt0 ev st_tgt1) ->
                             (ekind ev = observableE) /\
-                         exists st_src1, (src.(step) st_src0 ev st_src1) /\
+                         exists st_src1, (sem.(step) st_src0 ev st_src1) /\
                                       (_sim sim RR true true st_src1 st_tgt1))
       :
       sim_indC sim RR p_src p_tgt st_src0 st_tgt0
     | sim_indC_silentL
         st_src0 st_tgt
-        (SORT: ssort st_src0 = normal)
-        (SIM: exists ev st_src1, (src.(step) st_src0 ev st_src1) /\
+        (SORT: sort st_src0 = normal)
+        (SIM: exists ev st_src1, (sem.(step) st_src0 ev st_src1) /\
                               (ekind ev = silentE) /\
                          (sim RR true p_tgt st_src1 st_tgt))
       :
       sim_indC sim RR p_src p_tgt st_src0 st_tgt
     | sim_indC_silentR
         st_src st_tgt0
-        (SORT: tsort st_tgt0 = normal)
-        (SIM: forall ev st_tgt1, (tgt.(step) st_tgt0 ev st_tgt1) ->
+        (SORT: sort st_tgt0 = normal)
+        (SIM: forall ev st_tgt1, (sem.(step) st_tgt0 ev st_tgt1) ->
                             (ekind ev = silentE) /\
                          (sim RR p_src true st_src st_tgt1))
       :
       sim_indC sim RR p_src p_tgt st_src st_tgt0
     | sim_indC_ub
         st_src st_tgt
-        (UB: ssort st_src = undef)
+        (UB: sort st_src = undef)
       :
       sim_indC sim RR p_src p_tgt st_src st_tgt
     | sim_indC_progress
@@ -276,10 +291,10 @@ Section SIM.
   Qed.
 
   Variant sim_progressC
-          (sim: forall (RR: Z -> Z -> Prop), bool -> bool -> src.(state) -> tgt.(state) -> Prop)
+          (sim: forall (RR: Z -> Z -> Prop), bool -> bool -> sem.(state) -> sem.(state) -> Prop)
           (RR: Z -> Z -> Prop)
     :
-    bool -> bool -> src.(state) -> tgt.(state) -> Prop :=
+    bool -> bool -> sem.(state) -> sem.(state) -> Prop :=
     | sim_progressC_intro
         ps0 ps1 pt0 pt1 st_src st_tgt
         (SIM: sim RR ps1 pt1 st_src st_tgt)
@@ -322,19 +337,20 @@ End SIM.
 #[export] Hint Resolve sim_mon: paco.
 #[export] Hint Resolve cpn5_wcompat: paco.
 
-Definition simulation {l: Event} (src tgt: @STS l) := forall ps pt, sim (@eq Z) ps pt src.(init) tgt.(init).
+Definition simulation {l: Event} {sem: @STS l} (src tgt: Program sem) :=
+  forall ps pt, sim (@eq Z) ps pt src.(init) tgt.(init).
 
 Section ADEQ.
+  (** We can prove that the simulation is sound, i.e. the adequacy theorem holds. *)
 
   Context {event: Event}.
-  Context {src: @STS event}.
-  Context {tgt: @STS event}.
+  Context {sem: @STS event}.
 
   Lemma adequacy_spin
         (RR: Z -> Z -> Prop)
         ps pt
-        (st_src: src.(state))
-        (st_tgt: tgt.(state))
+        (st_src: sem.(state))
+        (st_tgt: sem.(state))
         (SIM: sim RR ps pt st_src st_tgt)
         (SPIN: diverge st_tgt)
     :
@@ -370,14 +386,14 @@ Section ADEQ.
   Qed.
 
   Lemma adequacy_aux
-        (st_src0: src.(state))
-        (st_tgt0: tgt.(state))
+        (st_src0: sem.(state))
+        (st_tgt0: sem.(state))
         ps pt
         (SIM: sim eq ps pt st_src0 st_tgt0)
     :
     forall tr, (behavior st_tgt0 tr) -> (behavior st_src0 tr).
   Proof.
-    revert_until tgt. ginit. gcofix CIH. i.
+    revert_until sem. ginit. gcofix CIH. i.
     move H0 before CIH. revert_until H0. induction H0 using @behavior_ind; ii.
     { generalize dependent retv. rename st into st_tgt0.
       induction SIM using @sim_ind; i; ss; clarify.
@@ -451,9 +467,10 @@ Section ADEQ.
   Qed.
 
   Theorem adequacy
+          (src tgt: Program sem)
           (SIM: simulation src tgt)
     :
-    refines tgt src.
+    refines src tgt.
   Proof.
     ii. eapply adequacy_aux; eauto.
     Unshelve. all: exact false.
