src/tutorial/Example2.v
@@ -1,0 +1,234 @@
+From sflib Require Import sflib.
+From Paco Require Import paco.
+From Tutorial Require Import Refinement.
+
+Set Implicit Arguments.
+
+Section SIM.
+  (** We will define a simulation relation that covers diverging programs.
+      This kind of simulations are called 'termination sensitive' or 'termination preserving'.
+      A correct definition involves coinduction and some nontrivial details.
+      So before we get to that, let us examine a *wrong* definition first 
+      and practice coinductive proofs.
+   *)
+
+  Context {event: Event}.
+  Context {sem: @STS event}.
+
+  Notation ekind := event.(label_kind).
+  Notation sort := sem.(state_sort).
+
+  (* This definition is almost the same as 'sim' defined in FiniteSimulation.v, 
+     but it is a coinductive definition, not an inductive one.
+   *)
+  Variant _sim
+          (sim: forall (RR: Z -> Z -> Prop), sem.(state) -> sem.(state) -> Prop)
+          (RR: Z -> Z -> Prop)
+    :
+    sem.(state) -> sem.(state) -> Prop :=
+    | sim_term
+        st_src st_tgt r_src r_tgt
+        (TERMS: sort st_src = final r_src)
+        (TERMT: sort st_tgt = final r_tgt)
+        (SIM: RR r_src r_tgt)
+      :
+      _sim sim RR st_src st_tgt
+    | sim_obs
+        st_src0 st_tgt0
+        (OBSS: sort st_src0 = normal)
+        (OBST: sort st_tgt0 = normal)
+        (SIM: forall ev st_tgt1,
+            (sem.(step) st_tgt0 ev st_tgt1) ->
+            (ekind ev = observableE) /\
+              exists st_src1, (sem.(step) st_src0 ev st_src1) /\
+                           (sim RR st_src1 st_tgt1))
+      :
+      _sim sim RR st_src0 st_tgt0
+    | sim_silentS
+        st_src0 st_tgt
+        (SORT: sort st_src0 = normal)
+        (SIM: exists ev st_src1,
+            (sem.(step) st_src0 ev st_src1) /\
+              (ekind ev = silentE) /\
+              (sim RR st_src1 st_tgt))
+      :
+      _sim sim RR st_src0 st_tgt
+    | sim_silentR
+        st_src st_tgt0
+        (SORT: sort st_tgt0 = normal)
+        (SIM: forall ev st_tgt1,
+            (sem.(step) st_tgt0 ev st_tgt1) ->
+            (ekind ev = silentE) /\
+              (sim RR st_src st_tgt1))
+      :
+      _sim sim RR st_src st_tgt0
+    | sim_ub
+        st_src st_tgt
+        (SORT: sort st_src = undef)
+      :
+      _sim sim RR st_src st_tgt.
+
+  Definition sim: forall (RR: Z -> Z -> Prop), sem.(state) -> sem.(state) -> Prop := paco3 _sim bot3.
+
+  Lemma sim_mon: monotone3 _sim.
+  Proof.
+    ii. inv IN.
+    - econs 1; eauto.
+    - econs 2; eauto. i. specialize (SIM _ _ H). des; eauto.
+    - econs 3; eauto. des; eauto. esplits; eauto.
+    - econs 4; eauto. i. specialize (SIM _ _ H). des; eauto.
+    - econs 5; eauto.
+  Qed.
+
+End SIM.
+#[local] Hint Constructors _sim: core.
+#[local] Hint Unfold sim: core.
+#[local] Hint Resolve sim_mon: paco.
+#[local] Hint Resolve cpn3_wcompat: paco.
+
+Definition simulation {l: Event} {sem: @STS l} (src tgt: Program sem) :=
+  sim (@eq Z) src.(init) tgt.(init).
+
+From Coq Require Import Strings.String List.
+From Tutorial Require Import Imp.
+
+Section EX.
+  (** Assuming that the above coinductive simulation is correct (i.e. adequacy theorem holds), 
+      we can prove refinement between possibly diverging programs. 
+   *)
+
+  Hypothesis adequacy: forall {l: Event} {sem: @STS l} (src tgt: Program sem),
+      simulation src tgt -> refines tgt src.
+
+  (* DIV2. Now we can prove the previous example, by coinduction. *)
+  Definition src6 : com :=
+    <{ "x" := 100;
+       while ("x")
+       do ("x" := AAny)
+       end;
+       ret "x"
+    }>.
+
+  Definition tgt6 : com :=
+    <{ "x" := 100;
+       while ("x")
+       do ("x" := AAny)
+       end;
+       ret "x"
+    }>.
+
+  (* Solves tgt undef case if tgt is not undef. *)
+  Ltac solve_tgt_ub := 
+    exfalso;
+    match goal with
+    | [UNDEF : forall _ _, ~ (ceval _ _ _) |- _] => eapply UNDEF
+    end;
+    repeat econs.
+
+  (* Makes a tgt step. *)
+  Ltac step_tgt_silent0 :=
+    match goal with
+    | [STEP: ceval _ _ _ |- _] => inv STEP
+    end;
+    ss; split; auto.
+
+  (* Combines above two tactics. *)
+  Ltac step_tgt_silent :=
+    try (pfold; econs 4;
+         [ss
+         | ss; intros ev st_tgt1 STEP0; inv STEP0;
+           [step_tgt_silent0; left | solve_tgt_ub]
+        ]).
+
+  (* Makes a src silent step. *)
+  Ltac step_src_silent :=
+    try (pfold; econs 3;
+         [ss
+         | ss; exists (inr LInternal); eexists; splits; ss; [repeat econs | left]
+        ]).
+
+  Goal refines (Imp_Program2 src6) (Imp_Program2 tgt6).
+  Proof.
+    apply adequacy. unfold simulation, Imp_Program2, Imp_STS2, src6, tgt6, Imp_init. ss.
+    (* We can use paco tactics to proceed. *)
+    pfold. econs 4. ss.
+    ss. i. inv H. 2: solve_tgt_ub. step_tgt_silent0. left.
+    (* Of course, we can make a tactic for this. *)
+    step_tgt_silent. inv H6. step_tgt_silent. step_tgt_silent.
+    (* The target reached a while loop. We take the source side to the loop too. *)
+    do 4 step_src_silent.
+    (* Now we start a coinductive proof. We first set up a coinductive hypothesis. *)
+    remember Reg.init as reg. clear Heqreg.
+    remember 100 as n. clear Heqn.
+    revert reg n. pcofix CIH. i.
+    (* Then make progress. *)
+    step_tgt_silent.
+    - (* False case; loop terminates. *)
+      clear CIH.
+      inv H6. inv H1.
+      do 2 step_src_silent.
+      do 2 step_tgt_silent.
+      inv H5. inv H1.
+      do 1 step_src_silent.
+      pfold. econs; ss.
+    - (* True case; loops. *)
+      rename H7 into TRUE. inv H6. inv H1.
+      step_tgt_silent.
+      inv H6.
+      step_tgt_silent.
+      (* Tactic 'step_src_silent' picks wrong constructor, so we prove manually. *)
+      pfold. econs 3; ss. do 2 eexists. splits.
+      { econs 1. eapply E_WhileTrue. repeat econs. auto. }
+      { ss. }
+      left.
+      (* AAny introduces nondeterminism. We picks what we need when AAny is in the src. *)
+      pfold. econs 3; ss. do 2 eexists. splits.
+      { econs 1. eapply E_Asgn. eapply (E_Any _ n). }
+      { ss. }
+      left.
+      (* Now we came back to the start of the while loop. We can end the proof by coinduction. *)
+      pfold. econs 3; ss. do 2 eexists. splits.
+      { repeat econs. }
+      { ss. }
+      right. eapply CIH.
+      Unshelve. exact 0.
+    - (* Leftover undef case. *)
+      exfalso. destruct (Z.eqb n 0) eqn:CASES.
+      + eapply UNDEF. eapply E_WhileFalse. repeat econs. apply Z.eqb_eq; auto.
+      + eapply UNDEF. eapply E_WhileTrue. repeat econs. apply Z.eqb_neq; auto.
+  Qed.
+
+
+  (** However, this simulation is *unsound*, and you can prove refinements that shouldn't hold.
+      In other words, the adequacy theorem does not hold.
+      Before we define a correct coinductive simulation, here are some counterexamples.
+   *)
+
+  (* CEX1. The src terminates, but the tgt diverges. Prove this by coinduction. *)
+  Definition src1 : com := <{ ret 0 }>.
+
+  Definition tgt1 : com :=
+    <{ while (1)
+       do skip
+       end;
+       ret 1
+    }>.
+
+  Goal refines (Imp_Program2 src1) (Imp_Program2 tgt1).
+  Proof.
+  Admitted.
+
+
+  (* CEX2. The other way around. Prove this by coinduction. *)
+  Goal refines (Imp_Program2 tgt1) (Imp_Program2 src1).
+  Proof.
+  Admitted.
+
+  (** These counterexamples show that we need a mechanism to prevent *infinite stuttering*.
+      Stuttering in simulation means that only one side (src or tgt) makes progress,
+      while the other side stutters at the same state.
+      Stuttering is an essential feature that allows scalable verifications.
+      Therefore, a correct and useful simulation should allow stuttering, but only finite times.
+   *)
+
+End EX.
